Sync

coq/theories/assembly/ASMSemantics.v
@@ -288,7 +288,7 @@ Definition can_write_mem_at (m : word64 -> option (option word64)) (a : word64) 
   exists v, m a = Some v.
 
 Definition memory_writable (r14 r15 : word64) (m : word64 -> option (option word64)) : Prop :=
-  word.ltu r14 r15 = true /\
+  (word.ltu r14 r15 = true \/ word.eqb r14 r15 = true) /\
   word.modu r14 (word.of_Z 4) = word.of_Z 0 /\
   word.modu r15 (word.of_Z 4) = word.of_Z 0 /\
   r14 <> word.of_Z 0 /\
